Simple praos block example.

praos/src/Praos/Impl.lean
@@ -8,31 +8,34 @@ namespace Praos.Impl
 
 structure PartyImpl where
   pid : Nat
-deriving DecidableEq
+deriving Repr, DecidableEq
 
 
 structure SortitionImpl where
-  isLeader : Slot → PartyImpl → Prop
+  schedule : List (Slot × PartyImpl)
 
-instance : @IsSortition PartyImpl SortitionImpl where
-  isLeader := SortitionImpl.isLeader
+instance instSortitionImpl : @IsSortition PartyImpl SortitionImpl where
+  isLeader so sl pa := so.schedule.elem ⟨sl, pa⟩
+
+variable {so : SortitionImpl}
 
 
 structure BlockHashImpl where
   val : Option (Nat × Nat)
-deriving Inhabited, DecidableEq
+deriving Repr, Inhabited, DecidableEq
 
 
 structure BlockImpl where
   slot : Slot
   creator : PartyImpl
   parent : BlockHashImpl
+deriving Repr
 
 private def hashBlock : BlockImpl → BlockHashImpl
 | ⟨sl, pa, _⟩ => BlockHashImpl.mk $ some ⟨sl, pa.pid⟩
 
-instance : @IsBlock PartyImpl BlockHashImpl _ BlockImpl where
-  create := BlockImpl.mk
+instance instBlockImpl (so : SortitionImpl) : @IsBlock PartyImpl SortitionImpl instSortitionImpl BlockHashImpl instInhabitedBlockHashImpl so BlockImpl where
+  create sl pa _ bh := BlockImpl.mk sl pa bh
   slot := BlockImpl.slot
   creator := BlockImpl.creator
   parent := BlockImpl.parent
@@ -41,6 +44,23 @@ instance : @IsBlock PartyImpl BlockHashImpl _ BlockImpl where
   create_slot := by simp [BlockImpl.mk]
   create_parent := by simp [BlockImpl.mk]
   not_genesis_hash := by simp [hashBlock, genesisBlockHash, Inhabited.default]
+
+namespace Example
+
+  def pax := PartyImpl.mk 1
+  def sox := SortitionImpl.mk [⟨1, pax⟩]
+  def bhx := BlockHashImpl.mk none
+
+  theorem h : instSortitionImpl.isLeader sox 1 pax := by
+    simp [IsSortition.isLeader, List.elem]
+    have _ : (1, pax) == (1, pax) := by rfl
+    simp [*]
+  #check h
+
+  def blx : BlockImpl := (instBlockImpl sox).create 1 pax h bhx
+  #eval blx
+
+end Example
 
 
 end Praos.Impl
